lib/misc.v
@@ -1,3 +1,5 @@
+From stdpp Require Export gmap.
+
 From iris.heap_lang Require Import notation.
 
 
@@ -6,3 +8,24 @@ Definition oloc_to_val (ol: option loc) : val :=
   | None => NONEV
   | Some l => SOMEV #l
   end.
+
+Local Open Scope Z.
+Definition node_rep : Type := Z * option loc * bool * val.
+Definition node_key (n: node_rep) : Z := n.1.1.1.
+Definition node_next (n: node_rep) : option loc := n.1.1.2.
+Definition node_mark (n: node_rep) : bool := n.1.2.
+Definition node_lock (n: node_rep) : val := n.2.
+
+Definition node_lt (x y: node_rep) : Prop := 
+  node_key x < node_key y.
+
+Definition rep_to_node (n: node_rep) : val :=
+  (#(node_key n), oloc_to_val (node_next n), #(node_mark n), (node_lock n)).
+
+Lemma fold_rep_to_node (n: node_rep) :
+  ((#(node_key n), oloc_to_val (node_next n), #(node_mark n), (node_lock n)))%V =
+  rep_to_node n.
+Proof. done. Qed.
+
+Definition key_equiv (S: gset node_rep) (S_keys: gset Z) :=
+  Permutation (elements S_keys) (map node_key (elements S)).
